Add proof sketch for GC

src/program_proof/mvcc/mvcc_ghost.v
@@ -1,24 +1,19 @@
 From Perennial.program_proof Require Import disk_prelude.
-From iris.algebra Require Import dfrac_agree gset.
+From iris.algebra Require Import dfrac_agree.
 From iris.algebra.lib Require Import mono_nat gmap_view.
 
-Local Definition key_fixedR := gmapR u64 (dfrac_agreeR (leibnizO nat)).
-Local Definition tidsR := gmap_viewR nat (leibnizO unit).
+Local Definition tidsR := gmap_viewR u64 (leibnizO unit).
 Local Definition sid_tidsR := gmapR u64 (dfrac_agreeR (leibnizO (gset u64))).
 
 Class mvcc_ghostG Σ :=
   {
-    (*
-    mvcc_ghost_dbmaps :> ghost_mapG Σ (nat * u64) u64;
-    mvcc_ghost_key_fixed :> inG Σ key_fixedR;
-    *)
     mvcc_active_tidsG :> inG Σ tidsR;
     mvcc_active_tids_siteG :> inG Σ sid_tidsR;
     mvcc_min_tidG :> inG Σ mono_natR;
   }.
 
 Definition mvcc_ghostΣ :=
-  #[(*ghost_mapΣ (nat * u64) u64; GFunctor key_fixedR;*)
+  #[
      GFunctor tidsR;
      GFunctor sid_tidsR;
      GFunctor mono_natR
@@ -30,11 +25,6 @@ Proof. solve_inG. Qed.
 
 Record mvcc_names :=
   {
-    (*
-    mvcc_dbmaps : gname;
-    mvcc_fixed : gname;
-    *)
-    (* XXX *)
     mvcc_active_tids_gn: gname;
     mvcc_active_tids_site_gn: gname;
     mvcc_min_tid_gn : gname
@@ -42,8 +32,6 @@ Record mvcc_names :=
 
 Section definitions.
 Context `{!heapGS Σ, !mvcc_ghostG Σ}.
-
-(* Definition tid_sentinel : nat := 18446744073709551615%nat. *)
 
 Definition mvccN := nroot .@ "mvcc_inv".
 
@@ -59,42 +47,30 @@ Admitted.
 Definition active_tids_auth γ tids : iProp Σ :=
   own γ.(mvcc_active_tids_gn) (gmap_view_auth (DfracOwn 1) tids).
 
-Definition active_tid γ (tid : nat) : iProp Σ :=
+Definition active_tid γ (tid : u64) : iProp Σ :=
   own γ.(mvcc_active_tids_gn) (gmap_view_frag (V:=leibnizO unit) tid (DfracOwn 1) tt).
 
 Definition active_tids_site γ (sid : u64) tids : iProp Σ :=
   own γ.(mvcc_active_tids_site_gn) {[sid := to_dfrac_agree (DfracOwn (1/2)) tids]}.
 
-Definition min_tid_auth γ tid : iProp Σ :=
-  own γ.(mvcc_min_tid_gn) (●MN tid).
+Definition min_tid_auth γ tidN : iProp Σ :=
+  own γ.(mvcc_min_tid_gn) (●MN tidN).
 
-Definition min_tid_lb γ tid : iProp Σ :=
-  own γ.(mvcc_min_tid_gn) (◯MN tid).
+Definition min_tid_lb γ tidN : iProp Σ :=
+  own γ.(mvcc_min_tid_gn) (◯MN tidN).
 
-Theorem active_ge_min γ tid tidlb :
+Theorem active_ge_min γ tid tidlbN :
   active_tid γ tid -∗
-  min_tid_lb γ tidlb -∗
-  ⌜(tid ≥ tidlb)%nat⌝.
+  min_tid_lb γ tidlbN -∗
+  ⌜(int.nat tid ≥ tidlbN)%nat⌝.
 Admitted.
 
-(*
-Definition fixed_ptsto γ (q : Qp) (key : u64) (fixed : nat) : iProp Σ :=
-  own γ.(mvcc_fixed) {[key := to_dfrac_agree (DfracOwn q) (fixed : (leibnizO _))]}.
-
-Definition db_ptsto γ (dq : dfrac) (ts : nat) (key : u64) (val : u64) : iProp Σ :=
-  (ts, key) ↪[γ.(mvcc_dbmaps)]{dq} val.
-*)
-
 Definition mvcc_invariant γ : iProp Σ :=
-  ∃ tidmin tidsactive,
-    min_tid_auth γ tidmin ∗
+  ∃ tidminN tidsactive,
+    min_tid_auth γ tidminN ∗
     active_tids_auth γ tidsactive ∗
     (* TODO: tidsactive is the union of tids of each *)
-    ⌜∀ tid, tid ∈ (dom (gset nat) tidsactive) -> (tid ≥ tidmin)%nat⌝.
-  (*
-  ∃ dbmaps,
-    ghost_map_auth γ.(mvcc_dbmaps) 1 dbmaps.
-  *)
+    ⌜∀ tid, tid ∈ (dom (gset u64) tidsactive) -> (int.nat tid ≥ tidminN)%nat⌝.
 
 Definition mvcc_inv γ : iProp Σ :=
   inv mvccN (mvcc_invariant γ).
